We shall have blockchain storage soon

Phi_Semantics/PhSem_BC_Storage.thy
@@ -1,14 +1,10 @@
 theory PhSem_BC_Storage
-  imports Phi_System.Resource_Template PhSem_MoV
+  imports PhSem_MoV PhSm_Addr
 begin
 
 section \<open>Semantics\<close>
 
-declare [[typedef_overloaded]]
-
-datatype contract = Null | Contract nat TY
-
-declare [[typedef_overloaded = false]]
+type_synonym contract = block
 
 setup \<open>Sign.mandatory_path "RES"\<close>
 
@@ -16,11 +12,25 @@ type_synonym storage = \<open>contract \<rightharpoonup> VAL discrete\<close>
 
 setup \<open>Sign.parent_path\<close>
 
-resource_space aggregate_mem =
-  aggregate_mem :: \<open>{h::RES.storage. finite (dom h) \<and> (\<forall>seg \<in> dom h. h seg \<in> Some ` discrete ` Well_Type (block.layout seg))}\<close>
-  (MoV_res Byte_Rep_of_Val \<open>block.layout\<close>)
+resource_space storage =
+  storage :: \<open>{h::RES.storage. finite (dom h) \<and> (\<forall>seg \<in> dom h. h seg \<in> Some ` discrete ` Well_Type (block.layout seg))}\<close>
+  (MoV_res \<open>id :: VAL \<Rightarrow> VAL\<close> \<open>block.layout\<close>)
   by (standard; simp)
 
+type_synonym contract_state = \<open>aggregate_path \<Rightarrow> VAL discrete share option\<close>
+
+fiction_space storage =
+  storage :: \<open>RES.storage.basic_fiction \<Zcomp>
+              \<F>_pointwise (\<lambda>blk.
+                  \<F>_functional (MovI.Rep_of_Val_ins (block.layout blk)) (MovI.Rep_of_Val_ins_dom (block.layout blk)) \<Zcomp>
+                  \<F>_functional ((\<circ>) to_share \<circ> Map_of_Val_ins) (Map_of_Val_ins_dom (block.layout blk)))\<close>
+     (perm_MoV_fiction RES.storage \<open>id :: VAL \<Rightarrow> VAL\<close> block.layout Null)
+  by (standard, auto simp add: MovI.Rep_of_Val_ins_def BI_eq_iff)
+
+
+\<phi>type_def Contract :: \<open>contract \<Rightarrow> (contract_state,'a) \<phi> \<Rightarrow> (fiction, 'a) \<phi>\<close> ("\<c>\<o>\<n>\<t>\<r>\<a>\<c>\<t>[_]")
+  where \<open>x \<Ztypecolon> Contract contract T \<equiv> x \<Ztypecolon> FIC.storage.\<phi> (contract \<^bold>\<rightarrow> T) \<s>\<u>\<b>\<j> contract \<noteq> Null\<close>
+  deriving Sep_Functor_1
 
 
 end
