Phi_Semantics/PhiSem_Mem_Pointer.thy
@@ -1,5 +1,5 @@
 theory PhiSem_Mem_Pointer
-  imports PhiSem_Mem_C_Base PhiSem_Agg_Void
+  imports PhiSem_Mem_C_Base PhSm_Addr
   keywords
       "\<tribullet>" :: quasi_command
   abbrevs "+_a" = "+\<^sub>a"
@@ -25,45 +25,6 @@ subsection \<open>Value\<close>
 
 subsubsection \<open>Formalization Definitions\<close>
 
-paragraph \<open>Base Representation for Logical and Physical Addresses\<close>
-
-declare [[typedef_overloaded]]
-datatype block = Null | Block nat TY
-
-setup \<open>Sign.mandatory_path "block"\<close>
-
-definition \<open>layout blk = (case blk of Null \<Rightarrow> \<v>\<o>\<i>\<d> | Block _ TY \<Rightarrow> TY)\<close>
-
-lemma layout[simp]:
-  \<open>block.layout Null = \<v>\<o>\<i>\<d>\<close>
-  \<open>block.layout (Block i TY) = TY\<close>
-  unfolding block.layout_def by simp+
-
-setup \<open>Sign.parent_path\<close>
-
-(*TODO: rename: block, offset*)
-datatype 'index addr = Addr (blk: block) (index: 'index)
-declare [[typedef_overloaded = false]]
-
-declare addr.sel[iff, \<phi>safe_simp]
-hide_const (open) blk index
-
-lemma split_memaddr_all: \<open>All P \<longleftrightarrow> (\<forall>blk ofs. P (Addr blk ofs))\<close> by (metis addr.exhaust) 
-lemma split_memaddr_ex : \<open>Ex P  \<longleftrightarrow> (\<exists>blk ofs. P (Addr blk ofs))\<close> by (metis addr.exhaust) 
-lemma split_memaddr_meta_all:
-  \<open>(\<And>x. PROP P x) \<equiv> (\<And>blk ofs. PROP P (Addr blk ofs))\<close>
-proof
-  fix blk ofs
-  assume \<open>\<And>x. PROP P x\<close>
-  then show \<open>PROP P (Addr blk ofs)\<close> .
-next
-  fix x
-  assume \<open>\<And>blk ofs. PROP P (Addr blk ofs)\<close>
-  note this[of \<open>addr.blk x\<close> \<open>addr.index x\<close>, simplified]
-  then show \<open>PROP P x\<close> .
-qed
-
-
 paragraph \<open>Address Space\<close>
 
 consts addrspace_bits :: "nat" \<comment> \<open>bit width of address space, in unit of bits\<close>
@@ -83,58 +44,11 @@ lemma unat_to_size_t[simp]:
   \<open>n < 2 ^ addrspace_bits \<Longrightarrow> unat (to_size_t n) = n\<close>
   by (simp add: of_nat_inverse)
 
-paragraph \<open>Logical and Physical Addresses\<close>
+paragraph \<open>Physical Addresses\<close>
 
-type_synonym address = "aggregate_path addr" \<comment> \<open>Logical address\<close>
 type_synonym rawaddr = \<open>\<s>\<i>\<z>\<e>_\<t> word addr\<close> \<comment> \<open>Physical pointer having physical offset\<close>
 
-
 subsubsection \<open>Algebraic Properties\<close>
-
-instantiation block :: zero begin
-definition [simp]: "zero_block = Null"
-instance ..
-end
-
-instantiation addr :: (zero) zero begin
-definition "zero_addr = (Addr 0 0)"
-instance ..
-end
-
-lemma memaddr_blk_zero[simp]:
-  \<open>addr.blk 0 = Null\<close>
-  unfolding zero_addr_def by simp
-
-lemma memaddr_idx_zero[simp]:
-  \<open>addr.index 0 = 0\<close>
-  unfolding zero_addr_def by simp
-
-
-paragraph \<open>Freshness\<close>
-
-lemma infinite_UNIV_int [simp]: "infinite (UNIV::int set)"
-proof
-  assume "finite (UNIV::int set)"
-  moreover have "inj (\<lambda>i::int. 2 * i)"
-    by (rule injI) simp
-  ultimately have "surj (\<lambda>i::int. 2 * i)"
-    by (rule finite_UNIV_inj_surj)
-  thm finite_UNIV_inj_surj
-  then obtain i :: int where "1 = 2 * i" by (rule surjE)
-  then show False by presburger
-qed
-
-lemma memblk_infinite[simp]:
-  \<open>infinite (UNIV :: block set)\<close>
-  using inj_on_finite[where A = \<open>UNIV::nat set\<close> and B = \<open>(UNIV :: block set)\<close>
-        and f = \<open>\<lambda>n. Block n undefined\<close>]
-  by (meson infinite_UNIV_char_0 injI block.inject top_greatest)
-
-lemma memblk_infinite_TY:
-  \<open>infinite {a. block.layout a = TY}\<close>
-  using inj_on_finite[where A = \<open>UNIV::nat set\<close> and B = \<open>{a. block.layout a = TY}\<close>
-        and f = \<open>\<lambda>n. Block n TY\<close>]
-  using inj_def by fastforce
 
 lemma Mem_freshness:
   \<open>finite (dom f) \<Longrightarrow> \<exists>k. f k = None \<and> block.layout k = TY \<and> k \<noteq> Null\<close>
@@ -165,13 +79,6 @@ abbreviation \<open>type_storable_in_mem T \<equiv> MemObj_Size T < 2^addrspace_
 
 
 subsubsection \<open>Validity of Mem Block and Addresses\<close>
-
-paragraph \<open>The type of the object that a pointer points to\<close>
-
-definition address_type :: \<open>address \<Rightarrow> TY\<close>
-  where \<open>address_type addr \<equiv> index_type (addr.index addr) (block.layout (addr.blk addr))\<close>
-
-adhoc_overloading Type_Of_syntax address_type
 
 definition \<open>Valid_MemBlk seg = (
     case seg of Null \<Rightarrow> True
